theories/RocqIRSem.v
@@ -1,0 +1,290 @@
+(** Semantics of the Rocq backend IR, and emit correctness for the core fragment.
+
+    We model [RocqExpr] as a small functional language [RVal]/[REval], then prove
+    that [emit_rocq_expr] on [CoreFrag] terms that are [CoreWT] produces IR that
+    evaluates to a value related to the expected Chester type. *)
+
+From Stdlib Require Import Strings.String.
+From Stdlib Require Import List.
+From Stdlib Require Import Bool.
+From Stdlib Require Import Arith.PeanoNat.
+Import ListNotations.
+Open Scope string_scope.
+
+Require Import Chester.AST.
+Require Import Chester.RocqAST.
+Require Import Chester.RocqBackend.
+Require Import Chester.CoreChecker.
+Require Import Chester.CoreTyping.
+
+(* ------------------------------------------------------------ *)
+(* Values and environments                                      *)
+(* ------------------------------------------------------------ *)
+
+Inductive RVal : Type :=
+| RVNat : nat -> RVal
+| RVBool : bool -> RVal
+| RVClo : string -> RocqExpr -> list (string * RVal) -> RVal
+| RVUnit : RVal.
+
+Definition REnv := list (string * RVal).
+
+Fixpoint rlookup (x : string) (env : REnv) : option RVal :=
+  match env with
+  | [] => None
+  | (k, v) :: rest =>
+      if String.eqb x k then Some v else rlookup x rest
+  end.
+
+(* ------------------------------------------------------------ *)
+(* Big-step evaluation on RocqExpr (core fragment)              *)
+(* ------------------------------------------------------------ *)
+
+Inductive REval : REnv -> RocqExpr -> RVal -> Prop :=
+| RE_Nat : forall env n,
+    REval env (RocqNat (nat_to_string n)) (RVNat n)
+| RE_Bool : forall env b,
+    REval env (RocqBool b) (RVBool b)
+| RE_Unit : forall env,
+    REval env RocqUnit RVUnit
+| RE_Id : forall env x v,
+    rlookup x env = Some v ->
+    REval env (RocqIdentifier x) v
+| RE_Lam : forall env x body,
+    REval env (RocqLam [x] body) (RVClo x body env)
+| RE_App : forall env f a x body envf va v,
+    REval env f (RVClo x body envf) ->
+    REval env a va ->
+    REval ((x, va) :: envf) body v ->
+    REval env (RocqApp f [a]) v
+| RE_IfT : forall env c t e v,
+    REval env c (RVBool true) ->
+    REval env t v ->
+    REval env (RocqIf c t e) v
+| RE_IfF : forall env c t e v,
+    REval env c (RVBool false) ->
+    REval env e v ->
+    REval env (RocqIf c t e) v.
+
+(* ------------------------------------------------------------ *)
+(* Semantic typing of IR values (logical relation on types)     *)
+(* ------------------------------------------------------------ *)
+
+Fixpoint RValTy (v : RVal) (ty : AST) {struct ty} : Prop :=
+  match ty with
+  | AstRef s =>
+      if String.eqb s "Integer" then
+        match v with RVNat _ => True | _ => False end
+      else if String.eqb s "Boolean" then
+        match v with RVBool _ => True | _ => False end
+      else False
+  | AstFunTy [] [(_, sigma)] tau [] =>
+      match v with
+      | RVClo x body env =>
+          forall va, RValTy va sigma ->
+            exists v', REval ((x, va) :: env) body v' /\ RValTy v' tau
+      | _ => False
+      end
+  | _ => False
+  end.
+
+Definition REnvTy (gamma : list (string * AST)) (env : REnv) : Prop :=
+  forall x ty, core_lookup x gamma = Some ty ->
+    exists v, rlookup x env = Some v /\ RValTy v ty.
+
+Lemma renv_ty_nil : REnvTy [] [].
+Proof. intros x ty H. discriminate H. Qed.
+
+Lemma renv_ty_cons : forall gamma env x sigma v,
+  REnvTy gamma env ->
+  RValTy v sigma ->
+  REnvTy ((x, sigma) :: gamma) ((x, v) :: env).
+Proof.
+  intros gamma env x sigma v Henv Hv y ty Hy.
+  unfold core_lookup in Hy; simpl in Hy.
+  destruct (String.eqb y x) eqn:Ey.
+  - inversion Hy; subst. exists v. split.
+    + simpl. rewrite Ey. reflexivity.
+    + exact Hv.
+  - destruct (Henv y ty Hy) as [v' [Hl Ht]].
+    exists v'. split.
+    + simpl. rewrite Ey. exact Hl.
+    + exact Ht.
+Qed.
+
+Lemma RValTy_nat : forall n, RValTy (RVNat n) CoreChecker.IntType.
+Proof.
+  intros n.
+  unfold CoreChecker.IntType, RValTy.
+  rewrite (String.eqb_refl "Integer").
+  exact I.
+Qed.
+
+Lemma RValTy_bool : forall b, RValTy (RVBool b) CoreChecker.BoolType.
+Proof.
+  intros b.
+  unfold CoreChecker.BoolType, RValTy.
+  destruct (String.eqb "Boolean" "Integer") eqn:E1.
+  - apply String.eqb_eq in E1. discriminate E1.
+  - rewrite (String.eqb_refl "Boolean"). exact I.
+Qed.
+
+Lemma RValTy_clo : forall x body env sigma tau,
+  (forall va, RValTy va sigma ->
+     exists v, REval ((x, va) :: env) body v /\ RValTy v tau) ->
+  RValTy (RVClo x body env) (CoreArrow sigma tau).
+Proof.
+  intros x body env sigma tau H.
+  unfold CoreArrow. simpl. exact H.
+Qed.
+
+Lemma RValTy_arrow_is_clo : forall v sigma tau,
+  RValTy v (CoreArrow sigma tau) ->
+  exists x body env, v = RVClo x body env /\
+    forall va, RValTy va sigma ->
+      exists v', REval ((x, va) :: env) body v' /\ RValTy v' tau.
+Proof.
+  intros v sigma tau H.
+  unfold CoreArrow in H. simpl in H.
+  destruct v; try contradiction.
+  exists s, r, l. split; [reflexivity|exact H].
+Qed.
+
+Lemma RValTy_bool_inv : forall v,
+  RValTy v CoreChecker.BoolType -> exists b, v = RVBool b.
+Proof.
+  intros v H.
+  unfold CoreChecker.BoolType, RValTy in H.
+  destruct (String.eqb "Boolean" "Integer") eqn:E1.
+  - apply String.eqb_eq in E1. discriminate E1.
+  - rewrite (String.eqb_refl "Boolean") in H.
+    destruct v; try contradiction. exists b. reflexivity.
+Qed.
+
+(* ------------------------------------------------------------ *)
+(* Emit shape lemmas                                            *)
+(* ------------------------------------------------------------ *)
+
+Lemma emit_int : forall n,
+  emit_rocq_expr (AstIntLit n) = RocqNat (nat_to_string n).
+Proof. reflexivity. Qed.
+
+Lemma emit_bool : forall b,
+  emit_rocq_expr (AstBoolLit b) = RocqBool b.
+Proof. reflexivity. Qed.
+
+Lemma emit_ref : forall x,
+  emit_rocq_expr (AstRef x) = RocqIdentifier x.
+Proof. reflexivity. Qed.
+
+Lemma emit_lam : forall x ty body,
+  emit_rocq_expr (AstLam x ty body) = RocqLam [x] (emit_rocq_expr body).
+Proof. reflexivity. Qed.
+
+Lemma emit_app1 : forall f a,
+  emit_rocq_expr (AstApp f [a]) =
+  RocqApp (emit_rocq_expr f) [emit_rocq_expr a].
+Proof. reflexivity. Qed.
+
+Lemma emit_if : forall c t e,
+  emit_rocq_expr (AstIf c t e) =
+  RocqIf (emit_rocq_expr c) (emit_rocq_expr t) (emit_rocq_expr e).
+Proof. reflexivity. Qed.
+
+Lemma emit_span : forall sp e,
+  emit_rocq_expr (AstSpan sp e) = emit_rocq_expr e.
+Proof. reflexivity. Qed.
+
+(* ------------------------------------------------------------ *)
+(* Emit correctness                                             *)
+(* ------------------------------------------------------------ *)
+
+Theorem emit_rocq_correct :
+  forall gamma e ty env,
+    CoreFrag e ->
+    CoreWT gamma e ty ->
+    REnvTy gamma env ->
+    exists v, REval env (emit_rocq_expr e) v /\ RValTy v ty.
+Proof.
+  intros gamma e ty env Hfrag.
+  revert gamma ty env.
+  induction Hfrag as
+    [ n
+    | b
+    | x
+    | x tyb b Hty IHty Hb IHb
+    | f a Hf IHf Ha IHa
+    | c t e Hc IHc Ht IHt He IHe
+    | sp e He IHe
+    ]; intros gamma ty env Hwt Henv.
+  - (* Int *)
+    inversion Hwt; subst.
+    exists (RVNat n). split; [rewrite emit_int; apply RE_Nat | apply RValTy_nat].
+  - (* Bool *)
+    inversion Hwt; subst.
+    exists (RVBool b). split; [rewrite emit_bool; apply RE_Bool | apply RValTy_bool].
+  - (* Ref *)
+    inversion Hwt; subst.
+    match goal with
+    | Hlook : core_lookup x gamma = Some ty |- _ =>
+        destruct (Henv x ty Hlook) as [v [Hl Ht']]
+    end.
+    exists v. split; [rewrite emit_ref; apply RE_Id; exact Hl | exact Ht'].
+  - (* Lam *)
+    inversion Hwt; subst.
+    exists (RVClo x (emit_rocq_expr b) env). split.
+    + rewrite emit_lam. apply RE_Lam.
+    + apply RValTy_clo. intros va Hva.
+      match goal with
+      | Hbody : CoreWT ((x, ?sigma) :: gamma) b ?tau0 |- _ =>
+          apply (IHb ((x, sigma) :: gamma) tau0 ((x, va) :: env) Hbody)
+      end.
+      apply renv_ty_cons; [exact Henv | exact Hva].
+  - (* App *)
+    inversion Hwt; subst.
+    match goal with
+    | Hfwt : CoreWT gamma f (CoreArrow ?sigma ?tau0),
+      Hawt : CoreWT gamma a ?sigma |- _ =>
+        destruct (IHf gamma _ env Hfwt Henv) as [vf [Ef Tf]];
+        destruct (IHa gamma _ env Hawt Henv) as [va [Ea Ta]];
+        destruct (RValTy_arrow_is_clo vf sigma tau0 Tf)
+          as [x0 [body [envf [Evf Hclo]]]];
+        rewrite Evf in Ef;
+        destruct (Hclo va Ta) as [v [Ev Tv]];
+        exists v; split; [| exact Tv];
+        rewrite emit_app1; eapply RE_App; [exact Ef | exact Ea | exact Ev]
+    end.
+  - (* If *)
+    inversion Hwt; subst.
+    match goal with
+    | Hcwt : CoreWT gamma c CoreChecker.BoolType,
+      Htwt : CoreWT gamma t ty,
+      Hewt : CoreWT gamma e ty |- _ =>
+        destruct (IHc gamma _ env Hcwt Henv) as [vc [Ec Tc]];
+        destruct (RValTy_bool_inv vc Tc) as [bv Eb];
+        rewrite Eb in Ec;
+        destruct bv;
+        [ destruct (IHt gamma ty env Htwt Henv) as [v [Ev Tv]];
+          exists v; split; [| exact Tv];
+          rewrite emit_if; eapply RE_IfT; [exact Ec | exact Ev]
+        | destruct (IHe gamma ty env Hewt Henv) as [v [Ev Tv]];
+          exists v; split; [| exact Tv];
+          rewrite emit_if; eapply RE_IfF; [exact Ec | exact Ev] ]
+    end.
+  - (* Span *)
+    inversion Hwt; subst.
+    match goal with
+    | Hinner : CoreWT gamma e ty |- _ =>
+        rewrite emit_span; apply (IHe gamma ty env Hinner Henv)
+    end.
+Qed.
+
+Corollary emit_rocq_correct_closed :
+  forall e ty,
+    CoreFrag e ->
+    CoreWT [] e ty ->
+    exists v, REval [] (emit_rocq_expr e) v /\ RValTy v ty.
+Proof.
+  intros e ty Hf Hw.
+  eapply emit_rocq_correct; [exact Hf | exact Hw | exact renv_ty_nil].
+Qed.
